CheckedArith.v
@@ -1,0 +1,306 @@
+From Coq Require Import ZArith Lia.
+From Vyper Require Import Config L10.UInt256 L10.AST.
+
+Local Open Scope Z_scope.
+
+
+(** Unchecked addition modulo [2^256]. *)
+Definition uint256_add {C: VyperConfig} (a b: uint256)
+: uint256
+:= uint256_of_Z (Z_of_uint256 a + Z_of_uint256 b).
+
+(** Checked [a + b] close to how it's compiled: [assert a + b >= a; a + b]. *)
+Definition uint256_checked_add {C: VyperConfig} (a: uint256) (b: uint256)
+: option uint256
+:= let result := uint256_add a b in
+   if Z_of_uint256 result >=? Z_of_uint256 a
+     then Some result
+     else None.
+
+Lemma uint256_checked_add_ok {C: VyperConfig} (a b: uint256):
+  uint256_checked_add a b = interpret_binop Add a b.
+Proof.
+cbn. unfold uint256_checked_add. unfold uint256_add.
+assert (A := uint256_range a).
+assert (B := uint256_range b).
+remember (Z_of_uint256 a) as x.
+remember (Z_of_uint256 b) as y.
+unfold maybe_uint256_of_Z.
+rewrite uint256_ok.
+assert (NN: 0 <= x + y) by lia.
+assert (D := Z.lt_ge_cases (x + y) (2 ^ 256)).
+case D; clear D; intro D.
+{ (* no overflow *)
+  rewrite (Z.mod_small (x + y) (2 ^ 256) (conj NN D)).
+  assert (G: x <= x + y) by lia.
+  rewrite<- Z.geb_le in G. rewrite G.
+  now rewrite Z.eqb_refl.
+}
+(* overflow *)
+assert (M: (x + y) mod 2 ^ 256 = x + y - 2 ^ 256).
+{
+  replace ((x + y) mod 2 ^ 256) with ((x + y + - 2 ^ 256) mod 2 ^ 256).
+  { apply Z.mod_small. lia. }
+  rewrite Z.add_mod by discriminate.
+  replace (- 2 ^ 256 mod 2 ^ 256) with 0 by trivial.
+  rewrite Z.add_0_r.
+  apply Z.mod_mod.
+  discriminate.
+}
+assert (F: (x + y) mod 2 ^ 256 >=? x = false).
+{ rewrite Z.geb_leb. rewrite Z.leb_gt. lia. }
+rewrite F.
+assert (F': (x + y) mod 2 ^ 256 =? x + y = false).
+{ rewrite Z.eqb_neq. lia. }
+now rewrite F'.
+Qed.
+
+
+(** Unchecked subtraction modulo [2^256]. *)
+Definition uint256_sub {C: VyperConfig} (a b: uint256)
+: uint256
+:= uint256_of_Z (Z_of_uint256 a - Z_of_uint256 b).
+
+(** Checked [a - b] close to how it's compiled: [assert a >= b; a - b]. *)
+Definition uint256_checked_sub {C: VyperConfig} (a b: uint256)
+: option uint256
+:= if Z_of_uint256 a >=? Z_of_uint256 b
+     then Some (uint256_sub a b)
+     else None.
+
+Lemma uint256_checked_sub_ok {C: VyperConfig} (a b: uint256):
+  uint256_checked_sub a b = interpret_binop Sub a b.
+Proof.
+cbn. unfold uint256_checked_sub. unfold uint256_sub.
+assert (A := uint256_range a).
+assert (B := uint256_range b).
+remember (Z_of_uint256 a) as x.
+remember (Z_of_uint256 b) as y.
+unfold maybe_uint256_of_Z.
+rewrite uint256_ok.
+rewrite Z.geb_leb.
+assert (D := Z.lt_ge_cases x y).
+case D; clear D; intro D.
+{ (* overflow *)
+  assert (F: (x - y) mod 2 ^ 256 =? x - y = false).
+  {
+    rewrite Z.eqb_neq. intro H.
+    apply Z.mod_small_iff in H. 2:discriminate.
+    lia.
+  }
+  rewrite F.
+  apply Z.leb_gt in D. now rewrite D.
+}
+(* no overflow *)
+assert (T: (x - y) mod 2 ^ 256 =? x - y = true).
+{ rewrite Z.eqb_eq. apply Z.mod_small. lia. }
+rewrite T.
+apply Z.leb_le in D. now rewrite D.
+Qed.
+
+
+(** Unchecked multiplication modulo [2^256]. *)
+Definition uint256_mul {C: VyperConfig} (a b: uint256)
+: uint256
+:= uint256_of_Z (Z_of_uint256 a * Z_of_uint256 b).
+
+(** Unchecked division modulo [2^256]. *)
+Definition uint256_div {C: VyperConfig} (a b: uint256)
+: uint256
+:= uint256_of_Z (Z_of_uint256 a / Z_of_uint256 b).
+
+(** As in EVM, [x / 0 = 0]. *)
+Lemma uint256_div_0_r {C: VyperConfig} (a: uint256):
+  uint256_div a zero256 = zero256.
+Proof.
+unfold uint256_div. unfold zero256.
+rewrite uint256_ok.
+now rewrite Zdiv_0_r.
+Qed.
+
+(** Checked [a * b] close to how it's compiled:
+     [if a == 0
+        then 0
+        else assert a * b / a = b;
+             a * b]. *)
+Definition uint256_checked_mul {C: VyperConfig} (a b: uint256)
+: option uint256
+:= if Z_of_uint256 a =? 0
+     then Some zero256
+     else let result := uint256_mul a b in
+          if Z_of_uint256 (uint256_div result a) =? Z_of_uint256 b
+            then Some result
+            else None.
+
+Lemma Z_div_le_l (a b: Z) (A: 0 <= a) (B: 0 <= b):
+  a / b <= a.
+Proof.
+apply Z.lt_eq_cases in B.
+case B; clear B; intro B.
+{
+  replace a with (a / 1) at 2 by apply Z.div_1_r.
+  apply Z.div_le_compat_l; lia.
+}
+subst b. rewrite Zdiv_0_r. exact A.
+Qed.
+
+Lemma uint256_checked_mul_ok {C: VyperConfig} (a: uint256) (b: uint256):
+  uint256_checked_mul a b = interpret_binop Mul a b.
+Proof.
+cbn. unfold uint256_checked_mul. unfold uint256_mul.
+unfold uint256_div.
+assert (A := uint256_range a).
+assert (B := uint256_range b).
+remember (Z_of_uint256 a) as x.
+remember (Z_of_uint256 b) as y.
+unfold maybe_uint256_of_Z.
+repeat rewrite uint256_ok.
+assert (D := Z.lt_ge_cases (x * y) (2 ^ 256)).
+case D; clear D; intro D.
+{ (* no overflow *)
+  replace ((x * y) mod 2 ^ 256) with (x * y).
+  2:{ symmetry. apply Z.mod_small. lia. }
+  remember (x =? 0) as x_zero. symmetry in Heqx_zero. destruct x_zero.
+  {
+    apply Z.eqb_eq in Heqx_zero. repeat rewrite Heqx_zero.
+    now repeat rewrite Z.mul_0_r.
+  }
+  rewrite Z.eqb_neq in Heqx_zero.
+  replace (x * y / x) with y.
+  2:{ rewrite Z.mul_comm. now rewrite (Z.div_mul y x Heqx_zero). }
+  replace (y mod 2 ^ 256) with y by now rewrite (Z.mod_small _ _ B).
+  now repeat rewrite Z.eqb_refl.
+}
+(* overflow *)
+remember (x =? 0) as x_zero. symmetry in Heqx_zero. destruct x_zero.
+{
+  apply Z.eqb_eq in Heqx_zero. rewrite Heqx_zero in D.
+  rewrite Z.mul_0_l in D. contradiction.
+}
+rewrite Z.eqb_neq in Heqx_zero.
+(* We're going to get rid of the last mod here:
+    ((x * y) mod 2 ^ 256 / x) mod 2 ^ 256
+*)
+assert (U: (x * y) mod 2 ^ 256 / x < 2 ^ 256).
+{
+  apply (Z.le_lt_trans _ ((x * y) mod 2 ^ 256)).
+  {
+    apply Z_div_le_l. 2:tauto.
+    apply Z.mod_bound_pos; lia.
+  }
+  apply Z.mod_bound_pos; lia.
+}
+assert (L: 0 <= (x * y) mod 2 ^ 256 / x).
+{
+  apply Z.div_pos. 2:lia.
+  apply Z.mod_bound_pos; lia.
+}
+replace (((x * y) mod 2 ^ 256 / x) mod 2 ^ 256)
+  with ((x * y) mod 2 ^ 256 / x).
+2:{ symmetry. apply Z.mod_small. tauto. }
+
+(* This is the main point of the proof. *)
+assert (NE: (x * y) mod 2 ^ 256 / x <> y).
+{
+  intro H.
+  assert (M: (x * y) mod 2 ^ 256 <= x * y - 2 ^ 256).
+  {
+    replace ((x * y) mod 2 ^ 256) with ((x * y + - 2 ^ 256) mod 2 ^ 256).
+    2:{
+      rewrite Z.add_mod by discriminate.
+      replace (- 2 ^ 256 mod 2 ^ 256) with 0 by trivial.
+      rewrite Z.add_0_r.
+      apply Z.mod_mod.
+      discriminate.
+    }
+    apply Z.mod_le.
+    lia.
+    easy.
+  }
+  assert (Y: (x * y) mod 2 ^ 256 < x * y - x) by lia.
+  replace (x * y - x) with (x * (y - 1)) in Y by lia.
+  enough (Q: (x * y) mod 2 ^ 256 / x <= x * (y - 1) / x).
+  {
+    replace (x * (y - 1) / x) with (y - 1) in Q. { lia. }
+    rewrite Z.mul_comm.
+    symmetry. apply Z.div_mul. assumption.
+  }
+  apply Z.div_le_mono; lia.
+}
+apply Z.eqb_neq in NE. rewrite NE.
+enough (R: (x * y) mod 2 ^ 256 =? x * y = false) by now rewrite R.
+apply Z.eqb_neq.
+rewrite Z.mod_small_iff.
+lia. discriminate.
+Qed.
+
+(** Checked [a / b] close to how it's compiled: [assert b; a / b] *)
+Definition uint256_checked_div {C: VyperConfig} (a b: uint256)
+: option uint256
+:= if Z_of_uint256 b =? 0
+     then None
+     else Some (uint256_div a b).
+
+(* This is almost trivial but there's an extra range check in the interpreter. *)
+Lemma uint256_checked_div_ok {C: VyperConfig} (a: uint256) (b: uint256):
+  uint256_checked_div a b = interpret_binop Quot a b.
+Proof.
+cbn. unfold uint256_checked_div. unfold uint256_div.
+assert (A := uint256_range a).
+assert (B := uint256_range b).
+remember (Z_of_uint256 a) as x.
+remember (Z_of_uint256 b) as y.
+remember (y =? 0) as y_zero. symmetry in Heqy_zero. destruct y_zero.
+{ trivial. }
+rewrite Z.eqb_neq in Heqy_zero.
+unfold maybe_uint256_of_Z.
+repeat rewrite uint256_ok.
+enough (Q: (x / y) mod 2 ^ 256 =? x / y = true)
+  by now rewrite Q.
+rewrite Z.eqb_eq. apply Z.mod_small.
+split. { apply Z.div_pos; lia. }
+apply Z.div_lt_upper_bound; lia.
+Qed.
+
+
+(** Unchecked mod. *)
+Definition uint256_mod {C: VyperConfig} (a b: uint256)
+: uint256
+:= uint256_of_Z (Z_of_uint256 a mod Z_of_uint256 b).
+
+(** As in EVM, [x % 0 = 0]. *)
+Lemma uint256_mod_0_r {C: VyperConfig} (a: uint256):
+  uint256_mod a zero256 = zero256.
+Proof.
+unfold uint256_mod. unfold zero256. rewrite uint256_ok. cbn.
+now rewrite Zmod_0_r.
+Qed.
+
+(** Checked [a % b] close to how it's compiled: [assert b; a % b] *)
+Definition uint256_checked_mod {C: VyperConfig} (a b: uint256)
+: option uint256
+:= if Z_of_uint256 b =? 0
+     then None
+     else Some (uint256_mod a b).
+
+(* This is almost trivial but there's an extra range check in the interpreter. *)
+Lemma uint256_checked_mod_ok {C: VyperConfig} (a: uint256) (b: uint256):
+  uint256_checked_mod a b = interpret_binop Mod a b.
+Proof.
+cbn. unfold uint256_checked_mod. unfold uint256_mod.
+assert (A := uint256_range a).
+assert (B := uint256_range b).
+remember (Z_of_uint256 a) as x.
+remember (Z_of_uint256 b) as y.
+remember (y =? 0) as y_zero. symmetry in Heqy_zero. destruct y_zero.
+{ trivial. }
+rewrite Z.eqb_neq in Heqy_zero.
+unfold maybe_uint256_of_Z.
+repeat rewrite uint256_ok.
+replace ((x mod y) mod 2 ^ 256) with (x mod y). { now rewrite Z.eqb_refl. }
+symmetry. apply Z.mod_small.
+enough (0 <= x mod y < y) by lia.
+apply Z.mod_pos_bound. lia.
+Qed.
+
+(* assert a <= (~1 >> b); a << b *)
